src/DY.Example.NSL.SecurityProperties.fst
@@ -37,7 +37,6 @@ val responder_authentication:
   )
 let responder_authentication tr i alice bob n_a n_b = ()
 
-#push-options "--z3rlimit 50"
 val n_a_secrecy:
   tr:trace -> alice:principal -> bob:principal -> n_a:bytes ->
   Lemma
@@ -51,25 +50,7 @@ val n_a_secrecy:
   )
   (ensures principal_corrupt tr alice \/ principal_corrupt tr bob)
 let n_a_secrecy tr alice bob n_a =
-  attacker_only_knows_publishable_values nsl_protocol_preds tr n_a;
-  introduce (exists sess_id n_b. typed_state_was_set tr nsl_session_label alice sess_id (InitiatorSentMsg3 bob n_a n_b <: nsl_session)) ==> (principal_corrupt tr alice \/ principal_corrupt tr bob) with _. (
-    eliminate exists sess_id n_b. typed_state_was_set tr nsl_session_label alice sess_id (InitiatorSentMsg3 bob n_a n_b <: nsl_session) returns _ with _. (
-      assert(event_triggered tr alice nsl_event_label (serialize nsl_event (Initiate1 alice bob n_a)))
-    )
-  );
-  introduce (exists sess_id n_b. typed_state_was_set tr nsl_session_label bob sess_id (ResponderReceivedMsg3 alice n_a n_b <: nsl_session)) ==> (principal_corrupt tr alice \/ principal_corrupt tr bob) with _. (
-    eliminate exists sess_id n_b. typed_state_was_set tr nsl_session_label bob sess_id (ResponderReceivedMsg3 alice n_a n_b <: nsl_session) returns _ with _. (
-      assert(
-        principal_corrupt tr alice \/ principal_corrupt tr bob \/
-        event_triggered tr alice nsl_event_label (serialize nsl_event (Initiate2 alice bob n_a n_b))
-      );
-      assert(
-        principal_corrupt tr alice \/ principal_corrupt tr bob \/
-        event_triggered tr alice nsl_event_label (serialize nsl_event (Initiate1 alice bob n_a))
-      )
-    )
-  )
-#pop-options
+  attacker_only_knows_publishable_values nsl_protocol_preds tr n_a
 
 val n_b_secrecy:
   tr:trace -> alice:principal -> bob:principal -> n_b:bytes ->
@@ -84,17 +65,4 @@ val n_b_secrecy:
   )
   (ensures principal_corrupt tr alice \/ principal_corrupt tr bob)
 let n_b_secrecy tr alice bob n_b =
-  attacker_only_knows_publishable_values nsl_protocol_preds tr n_b;
-  introduce (exists sess_id n_a. typed_state_was_set tr nsl_session_label bob sess_id (ResponderReceivedMsg3 alice n_a n_b <: nsl_session)) ==> (principal_corrupt tr alice \/ principal_corrupt tr bob) with _. (
-    eliminate exists sess_id n_a. typed_state_was_set tr nsl_session_label bob sess_id (ResponderReceivedMsg3 alice n_a n_b <: nsl_session) returns _ with _. (
-      assert(event_triggered tr bob nsl_event_label (serialize nsl_event (Respond1 alice bob n_a n_b)))
-    )
-  );
-  introduce (exists sess_id n_a. typed_state_was_set tr nsl_session_label alice sess_id (InitiatorSentMsg3 bob n_a n_b <: nsl_session)) ==> (principal_corrupt tr alice \/ principal_corrupt tr bob) with _. (
-    eliminate exists sess_id n_a. typed_state_was_set tr nsl_session_label alice sess_id (InitiatorSentMsg3 bob n_a n_b <: nsl_session) returns _ with _. (
-      assert(
-        principal_corrupt tr alice \/ principal_corrupt tr bob \/
-        event_triggered tr bob nsl_event_label (serialize nsl_event (Respond1 alice bob n_a n_b))
-      )
-    )
-  )
+  attacker_only_knows_publishable_values nsl_protocol_preds tr n_b
